StrictPositivityPull.v
@@ -52,13 +52,57 @@ Opaque Nat.eq_dec.
 Opaque reducible_values.
 Opaque strictly_positive.
 
+Lemma cons_app:
+  forall X (x: X) (xs: list X),
+    x :: xs = (x :: nil) ++ xs.
+Proof.
+  steps.
+Qed.
+
 Lemma strictly_positive_pull_forall:
-  forall T theta A B v X a,
+  forall T theta A B v X,
     ~(X ∈ pfv T type_var) ->
-    non_empty theta A ->
+    twf A 0 ->
+    twf B 0 ->
+    twf T 1 ->
+    wf A 0 ->
+    wf B 1 ->
+    wf T 0 ->
+    is_erased_type A ->
+    is_erased_type T ->
+    valid_interpretation theta ->
     strictly_positive (topen 0 T (fvar X type_var)) (X :: nil) ->
     reducible_values theta v (topen 0 T (T_forall A B)) ->
-    reducible_values theta a A ->
-    reducible_values theta v (topen 0 T (open 0 B a)).
+    forall a,
+      reducible_values theta a A ->
+      reducible_values theta v (topen 0 T (open 0 B a)).
 Proof.
-Admitted.
+  steps.
+  apply reducibility_subst_head with
+    (makeFresh (
+       pfv T type_var ::
+       pfv A type_var ::
+       pfv B type_var ::
+       pfv (open 0 B a) type_var ::
+       nil
+    ));
+    repeat step || t_listutils || apply twf_open || apply wf_open;
+    try finisher;
+      eauto with btwf;
+      eauto with bwf.
+
+  rewrite cons_app.
+  lazymatch goal with
+  | H: wf ?B 1 |- reducible_values (((?X,?RC) :: nil) ++ ?theta) ?v ?T =>
+    eapply strictly_positive_push_forall with
+      ((X, fun a2 v => reducible_values theta v (T_forall A B)) :: nil) A
+  end;
+    repeat step || apply wf_topen || apply twf_topen || unfold non_empty ||
+           apply is_erased_type_topen || t_listutils || simp_red ||
+           apply reducibility_subst_head2 || t_instantiate_reducible ||
+           (eapply strictly_positive_rename_one; eauto);
+    eauto;
+    try finisher;
+    eauto using reducibility_is_candidate;
+    eauto with berased.
+Qed.
