StrictPositivityPush.v
@@ -56,10 +56,46 @@ Lemma strictly_positive_push_forall2:
   forall T theta A B v X,
     ~(X ∈ pfv T type_var) ->
     non_empty theta A ->
+    twf A 0 ->
+    twf B 0 ->
+    twf T 1 ->
+    wf A 0 ->
+    wf B 1 ->
+    wf T 0 ->
+    is_erased_type A ->
+    is_erased_type T ->
+    valid_interpretation theta ->
     strictly_positive (topen 0 T (fvar X type_var)) (X :: nil) ->
     (forall a,
         reducible_values theta a A ->
         reducible_values theta v (topen 0 T (open 0 B a))) ->
     reducible_values theta v (topen 0 T (T_forall A B)).
 Proof.
-Admitted.
+  intros; t_instantiate_non_empty; repeat step.
+  apply reducibility_subst_head with
+    (makeFresh (
+       pfv T type_var ::
+       pfv A type_var ::
+       pfv B type_var ::
+       nil
+    ));
+    repeat step || t_listutils;
+    try finisher.
+
+  rewrite cons_app.
+  match goal with
+  | H: wf ?B 1 |- reducible_values (((?X,?RC) :: nil) ++ ?theta) ?v ?T =>
+    eapply strictly_positive_push_forall with
+      ((X, fun a v => reducible_values theta v (open 0 B a)) :: nil) A
+  end; eauto;
+    repeat step || apply wf_topen || apply twf_topen || apply is_erased_type_topen ||
+           t_fv_open || t_listutils || apply wf_open || apply twf_open ||
+           t_instantiate_reducible || apply reducibility_subst_head2 || simp_red || t_closing;
+    eauto using reducibility_is_candidate with b_valid_interp;
+    try finisher;
+    eauto with btwf;
+    eauto with bwf.
+
+  - eapply strictly_positive_rename_one; eauto; steps; try finisher.
+  - rewrite (is_erased_term_tfv a0) in *; (steps; eauto with berased).
+Qed.
